\documentclass[a4paper, 12pt]{paper}
\input{../include/preamble}

\begin{document}
{\noindent
  v 2 \\
{\large\textbf{Generalized Rules of $\ldl$}}
}
\\

\begin{lem}
  $\ldl \not \vdash \{ A_i \to B_i \}_{i \in I} \Rightarrow$ for any finite set $I$.
\end{lem}
\begin{proof}
  First notice that $\ldl \not \vdash A \to B \Rightarrow$ for any $A$ and $B$, since no rule can derive the implication on the antecedent other that $LW$ over the empty sequent $\Rightarrow$, whose provability implies inconsistency of $\ldl$. It follows that $\ldl \not \vdash \{ A_i \to B_i \}_{i \in I} \Rightarrow$ for any $\{n_i\}$, $\{ A_i \}$ and $\{ B_i \}$ easily by induction on the size of $I$ and using $LW$.
\end{proof}

\begin{thm}
  Let $I$ be a finite (possibly empty) set, $\{ n_i \}_{i \in I}$ be a finite sequence of natural numbers and $m \ge 1$ be a natural number. If $\ldl \vdash \{ \nabla^{n_i} (A_i \to B_i) \}_{i \in I} \Rightarrow \nabla^m (C \to D)$, then either of the following holds:
  \begin{enumerate}
    \item There is $J \subseteq I$ and $k \in J$ such that $n_k \ge 1$ and $\ldl \vdash \{ \nabla^n_j (A_j \to B_j) \}_{j \in j} \Rightarrow \nabla^{n_k - 1} A_k$.
    \item For all $i \in I$ we have $n_i \ge 1$ and $\ldl \vdash \{ \nabla^{n_i - 1} (A_i \to B_i) \}_{i \in I} \Rightarrow \nabla^{m - 1} (C \to D)$.
  \end{enumerate}
\end{thm}
\begin{proof}


  By induction on the proof-tree for $\{ \nabla^{n_i} (A_i \to B_i) \}_{i \in I} \Rightarrow \nabla^m (C \to D)$. Observe that this proof-tree cannot end with any of the axioms or the logical rules other that $L \to$. The cases for $L \to$ and $N$ are trivial. So we consider the cases where the proof-tree ends with $LW$ or $Rw$. 

  In the case for $LW$ we have a proof-tree for $\{ \nabla^{n_i} (A_i \to B_i) \}_{i \in I'} \Rightarrow \nabla^m (C \to D)$ for some $I' \subseteq I$. We use induction hypothesis and thus, we have two sub-cases:
  \begin{enumerate}
    \item $\ldl \vdash \{ \nabla^{n_j} (A_j \to B_j) \}_{j \in J} \Rightarrow \nabla^{n_k - 1} A_k$ for some $J \subseteq I'$ and some $k \in J$ such that $n_k \ge 1$, which is the desired result.
    \item $\ldl \vdash \{ \nabla^{n_i - 1} (A_i \to B_i) \}_{i \in I'} \Rightarrow \nabla^{m - 1} (C \to D)$, and $n_i \ge 1$ for all $i \in I'$. In this case, use $LW$ again to reach $\{ \nabla^{n_i - 1} (A_i \to B_i) \}_{i \in I} \Rightarrow \nabla^{m - 1} (C \to D)$.
  \end{enumerate}

  In the case for $Rw$, where we have a proof-tree for $\{ \nabla^{n_i} (A_i \to B_i) \}_{i \in I'} \Rightarrow$, pick some $k \in I$ such that $n_{k} \ge 1$ and add it to the antecedent using $Rw$ to reach $\{ \nabla^{n_i} (A_i \to B_i) \}_{i \in J} \Rightarrow \nabla^{n_k - 1} A_k$. The previous Lemma guarantees that such $k$ exists.
\end{proof}

\end{document}
