First, observe that

\begin{prooftree}
	\AXC{}
	\RightLabel{$Ta$}
	\UIC{$\nabla (\top \rightarrow C) \Rightarrow \top$}

	\AXC{}
	\RightLabel{$(Id)$}
	\UIC{$\nabla (\top \rightarrow C), C \Rightarrow C$}

	\RightLabel{$L \rightarrow$}
	\BIC{$\nabla (\top \rightarrow C) \Rightarrow C$}
\end{prooftree}


Now, let $\D$ be the proof-tree above with $C = \nabla A \vee \nabla B$.

\begin{prooftree}
	\AXC{}
	\RightLabel{$(Id)$}
	\UIC{$\nabla A \Rightarrow \nabla A$}
	\RightLabel{$R\vee_1$}
	\UIC{$\nabla A \Rightarrow \nabla A \vee \nabla B$}
	\RightLabel{$Lw$}
	\UIC{$\nabla A , \top \Rightarrow \nabla A \vee \nabla B$}
	\RightLabel{$R \rightarrow$}
	\UIC{$A \Rightarrow \top \rightarrow (\nabla A \vee \nabla B)$}

	\AXC{}
	\RightLabel{$(Id)$}
	\UIC{$\nabla B \Rightarrow \nabla B$}
	\RightLabel{$R\vee_2$}
	\UIC{$\nabla B \Rightarrow \nabla A \vee \nabla B$}
	\RightLabel{$Lw$}
	\UIC{$\nabla B , \top \Rightarrow \nabla A \vee \nabla B$}
	\RightLabel{$R \rightarrow$}
	\UIC{$B \Rightarrow \top \rightarrow (\nabla A \vee \nabla B)$}

	\RightLabel{$L\vee$}
	\BIC{$A \vee B \Rightarrow \top \rightarrow (\nabla A \vee \nabla B)$}
	\RightLabel{$N$}
	\UIC{$\nabla (A \vee B) \Rightarrow \nabla (\top \rightarrow (\nabla A \vee \nabla B))$}

	\AXC{$\D$}

	\RightLabel{$cut$}
	\BIC{$\nabla (A \vee B) \Rightarrow \nabla A \vee \nabla B$}
\end{prooftree}

Call this proof-tree $\D_1$. Construct $\D_n$ inductively as follows.

\begin{prooftree}
	\AXC{$\mathcal{D}_{n-1}$}
	\noLine
	\UIC{$\nabla^{n-1} (A \vee B) \Rightarrow \nabla^{n-1} A \vee \nabla^{n-1} B$}
	\RightLabel{$N$}
	\UIC{$\nabla^n (A \vee B) \Rightarrow \nabla (\nabla^{n-1} A \vee \nabla^{n-1} B)$}

	\AXC{$\mathcal{D}_1$}
	\noLine
	\UIC{$\nabla (\nabla^{n-1} A \vee \nabla^{n-1} B) \Rightarrow \nabla^n A \vee \nabla^n B$}
	
	\RightLabel{$cut$} \LeftLabel{$\mathcal{D}_n:$}
	\BIC{$\nabla^n (A \vee B) \Rightarrow \nabla^n A \vee \nabla^n B$}
\end{prooftree}